spec/sail/lean/Out.lean
@@ -28,7 +28,7 @@ open CompareOp
 open BranchRegisterExecutionTarget
 open BarrierExecutionTarget
 
-/-- Type quantifiers: k_ex25288_ : Bool, k_ex25287_ : Bool -/
+/-- Type quantifiers: k_ex25308_ : Bool, k_ex25307_ : Bool -/
 def neq_bool (x : Bool) (y : Bool) : Bool :=
   (! (x == y))
 
@@ -178,7 +178,7 @@ def ConditionHolds (cond : (BitVec 4)) (nzcv : (BitVec 4)) : Bool :=
   then (! result)
   else result
 
-/-- Type quantifiers: k_ex25472_ : Bool, k_ex25471_ : Bool, k_datasize : Nat, k_datasize ∈
+/-- Type quantifiers: k_ex25492_ : Bool, k_ex25491_ : Bool, k_datasize : Nat, k_datasize ∈
   {32, 64} -/
 def integer_conditional_select (condition : (BitVec 4)) (nzcv : (BitVec 4)) (else_inc : Bool) (else_inv : Bool) (operand1 : (BitVec k_datasize)) (operand2 : (BitVec k_datasize)) : (BitVec k_datasize) :=
   let result : (BitVec k_datasize) := operand2
@@ -194,7 +194,7 @@ def integer_conditional_select (condition : (BitVec 4)) (nzcv : (BitVec 4)) (els
     then (BitVec.addInt result 1)
     else result)
 
-/-- Type quantifiers: k_ex25488_ : Bool, k_datasize : Nat, k_datasize ∈ {32, 64} -/
+/-- Type quantifiers: k_ex25508_ : Bool, k_datasize : Nat, k_datasize ∈ {32, 64} -/
 def integer_conditional_compare_register (condition : (BitVec 4)) (nzcv : (BitVec 4)) (flags__arg : (BitVec 4)) (operand1 : (BitVec k_datasize)) (operand2__arg : (BitVec k_datasize)) (sub_op : Bool) : (BitVec 4) :=
   let flags : (BitVec 4) := flags__arg
   let operand2 : (BitVec k_datasize) := operand2__arg
@@ -339,7 +339,7 @@ def vector_transfer_integer_dup (datasize : Nat) (elements : Nat) (esize : Nat) 
     loop_vars := (aset_Elem result e esize element)
   (pure loop_vars)
 
-/-- Type quantifiers: k_ex25627_ : Bool, datasize : Nat, elements : Nat, esize : Nat, esize ≥ 1
+/-- Type quantifiers: k_ex25647_ : Bool, datasize : Nat, elements : Nat, esize : Nat, esize ≥ 1
   ∧ elements ≥ 1 ∧ (elements * esize) = datasize -/
 def vector_arithmetic_binary_uniform_add_wrapping_single (datasize : Nat) (elements : Nat) (esize : Nat) (operand1 : (BitVec datasize)) (operand2 : (BitVec datasize)) (sub_op : Bool) : (BitVec datasize) := Id.run do
   let result : (BitVec datasize) := (Zeros datasize)
@@ -362,7 +362,7 @@ def vector_arithmetic_binary_uniform_add_wrapping_single (datasize : Nat) (eleme
     (pure loop_vars) ) : Id ((BitVec esize) × (BitVec esize) × (BitVec datasize)) )
   (pure result)
 
-/-- Type quantifiers: k_ex25695_ : Bool, k_ex25694_ : Bool, datasize : Nat, elements : Nat, esize :
+/-- Type quantifiers: k_ex25715_ : Bool, k_ex25714_ : Bool, datasize : Nat, elements : Nat, esize :
   Nat, esize ≥ 1 ∧ elements ≥ 1 ∧ (elements * esize) = datasize -/
 def vector_arithmetic_binary_uniform_maxmin_single (datasize : Nat) (elements : Nat) (esize : Nat) (operand1 : (BitVec datasize)) (operand2 : (BitVec datasize)) (minimum : Bool) (is_unsigned : Bool) : (BitVec datasize) := Id.run do
   let result : (BitVec datasize) := (Zeros datasize)
@@ -387,7 +387,7 @@ def vector_arithmetic_binary_uniform_maxmin_single (datasize : Nat) (elements : 
     (pure loop_vars) ) : Id (Int × Int × Int × (BitVec datasize)) )
   (pure result)
 
-/-- Type quantifiers: k_ex25746_ : Bool, k_ex25745_ : Bool, datasize : Nat, elements : Nat, esize :
+/-- Type quantifiers: k_ex25766_ : Bool, k_ex25765_ : Bool, datasize : Nat, elements : Nat, esize :
   Nat, esize ≥ 1 ∧ elements ≥ 1 ∧ (elements * esize) = datasize -/
 def vector_arithmetic_binary_uniform_cmp_int (cmp_eq : Bool) (datasize : Nat) (elements : Nat) (esize : Nat) (operand1 : (BitVec datasize)) (operand2 : (BitVec datasize)) (is_unsigned : Bool) : (BitVec datasize) := Id.run do
   let result : (BitVec datasize) := (Zeros datasize)
@@ -416,7 +416,7 @@ def vector_arithmetic_binary_uniform_cmp_int (cmp_eq : Bool) (datasize : Nat) (e
     (pure loop_vars) ) : Id (Int × Int × (BitVec datasize) × Bool) )
   (pure result)
 
-/-- Type quantifiers: k_ex25792_ : Bool, datasize : Nat, elements : Nat, esize : Nat, esize ≥ 1
+/-- Type quantifiers: k_ex25812_ : Bool, datasize : Nat, elements : Nat, esize : Nat, esize ≥ 1
   ∧ elements ≥ 1 ∧ (elements * esize) = datasize -/
 def vector_arithmetic_binary_uniform_cmp_bitwise (and_test : Bool) (datasize : Nat) (elements : Nat) (esize : Nat) (operand1 : (BitVec datasize)) (operand2 : (BitVec datasize)) : (BitVec datasize) := Id.run do
   let result : (BitVec datasize) := (Zeros datasize)
@@ -495,7 +495,7 @@ def vector_arithmetic_unary_cmp_int_bulk (comparison : CompareOp) (datasize : Na
     (pure loop_vars) ) : Id (Int × (BitVec datasize) × Bool) )
   (pure result)
 
-/-- Type quantifiers: k_ex25921_ : Bool, datasize : Nat, elements : Nat, esize : Nat, esize ≥ 1
+/-- Type quantifiers: k_ex25941_ : Bool, datasize : Nat, elements : Nat, esize : Nat, esize ≥ 1
   ∧ elements ≥ 1 ∧ (elements * esize) = datasize -/
 def vector_arithmetic_binary_uniform_sub_saturating (datasize : Nat) (elements : Nat) (esize : Nat) (operand1 : (BitVec datasize)) (operand2 : (BitVec datasize)) (is_unsigned : Bool) : (BitVec datasize) := Id.run do
   let result : (BitVec datasize) := (Zeros datasize)
@@ -518,7 +518,7 @@ def vector_arithmetic_binary_uniform_sub_saturating (datasize : Nat) (elements :
     (pure loop_vars) ) : Id (Int × Int × Int × (BitVec datasize)) )
   (pure result)
 
-/-- Type quantifiers: k_ex25972_ : Bool, shift : Int, k_ex25970_ : Bool, k_ex25969_ : Bool, datasize
+/-- Type quantifiers: k_ex25992_ : Bool, shift : Int, k_ex25990_ : Bool, k_ex25989_ : Bool, datasize
   : Nat, elements : Nat, esize : Nat, esize ≥ 1 ∧
   elements ≥ 1 ∧ (elements * esize) = datasize -/
 def vector_shift_right (accumulate : Bool) (datasize : Nat) (elements : Nat) (esize : Nat) (operand : (BitVec datasize)) (accumulator : (BitVec datasize)) (round : Bool) (shift : Int) (is_unsigned : Bool) : (BitVec datasize) := Id.run do
@@ -548,7 +548,7 @@ def vector_shift_right (accumulate : Bool) (datasize : Nat) (elements : Nat) (es
     (pure loop_vars) ) : Id (Int × (BitVec datasize)) )
   (pure result)
 
-/-- Type quantifiers: k_ex26025_ : Bool, datasize : Nat, elements : Nat, elements ≥ 1 ∧
+/-- Type quantifiers: k_ex26045_ : Bool, datasize : Nat, elements : Nat, elements ≥ 1 ∧
   (elements * 8) = datasize ∧ datasize ≤ 128 -/
 def vector_transfer_vector_table (datasize : Nat) (elements : Nat) (is_tbl : Bool) (indices : (BitVec datasize)) (table : (BitVec 128)) (dst : (BitVec datasize)) : (BitVec datasize) := Id.run do
   let result : (BitVec datasize) :=
@@ -572,7 +572,7 @@ def vector_transfer_vector_extract (datasize : Nat) (hi : (BitVec datasize)) (lo
   let concat : (BitVec (2 * datasize)) := (hi +++ lo)
   (BitVec.slice concat position datasize)
 
-/-- Type quantifiers: k_ex26057_ : Bool, k_ex26056_ : Bool, datasize : Nat, elements : Nat, esize :
+/-- Type quantifiers: k_ex26077_ : Bool, k_ex26076_ : Bool, datasize : Nat, elements : Nat, esize :
   Nat, esize ≥ 1 ∧ elements ≥ 1 ∧ (elements * esize) = datasize -/
 def vector_reduce_intmax (datasize : Nat) (elements : Nat) (esize : Nat) (operand : (BitVec datasize)) (min : Bool) (is_unsigned : Bool) : (BitVec esize) := Id.run do
   let maxmin : Int := 0
@@ -628,7 +628,7 @@ def num_of_LogicalOp (arg_ : LogicalOp) : Int :=
   | .LogicalOp_EOR => 1
   | .LogicalOp_ORR => 2
 
-/-- Type quantifiers: k_ex26115_ : Bool, datasize : Nat, datasize ≥ 1 -/
+/-- Type quantifiers: k_ex26135_ : Bool, datasize : Nat, datasize ≥ 1 -/
 def vector_arithmetic_binary_uniform_logical_andorr (datasize : Nat) (invert : Bool) (operand1 : (BitVec datasize)) (operand2__arg : (BitVec datasize)) (op : LogicalOp) : (BitVec datasize) :=
   let operand2 : (BitVec datasize) := operand2__arg
   let result : (BitVec datasize) := (Zeros datasize)
@@ -701,7 +701,7 @@ def FPNeg (op : (BitVec k_N)) : (BitVec k_N) :=
 def FPAbs (op : (BitVec k_N)) : (BitVec k_N) :=
   (0#1 +++ (BitVec.slice op 0 ((Sail.BitVec.length op) -i 1)))
 
-/-- Type quantifiers: k_ex26274_ : Bool, datasize : Nat, elements : Nat, esize : Nat, esize ∈
+/-- Type quantifiers: k_ex26294_ : Bool, datasize : Nat, elements : Nat, esize : Nat, esize ∈
   {32, 64} ∧ elements ≥ 1 ∧ (elements * esize) = datasize -/
 def vector_arithmetic_binary_uniform_add_fp (datasize : Nat) (elements : Nat) (esize : Nat) (operand1 : (BitVec datasize)) (operand2 : (BitVec datasize)) (fpcr : (BitVec 32)) (pair : Bool) : (BitVec datasize) := Id.run do
   let result : (BitVec datasize) := (Zeros datasize)
@@ -731,7 +731,7 @@ def vector_arithmetic_binary_uniform_add_fp (datasize : Nat) (elements : Nat) (e
     (pure loop_vars) ) : Id ((BitVec esize) × (BitVec esize) × (BitVec datasize)) )
   (pure result)
 
-/-- Type quantifiers: k_ex26381_ : Bool, datasize : Nat, elements : Nat, esize : Nat, esize ∈
+/-- Type quantifiers: k_ex26401_ : Bool, datasize : Nat, elements : Nat, esize : Nat, esize ∈
   {32, 64} ∧ elements ≥ 1 ∧ (elements * esize) = datasize -/
 def vector_arithmetic_binary_uniform_sub_fp (datasize : Nat) (elements : Nat) (esize : Nat) (operand1 : (BitVec datasize)) (operand2 : (BitVec datasize)) (fpcr : (BitVec 32)) (abs : Bool) : (BitVec datasize) := Id.run do
   let result : (BitVec datasize) := (Zeros datasize)
@@ -779,7 +779,7 @@ def vector_arithmetic_binary_uniform_mul_fp_product (datasize : Nat) (elements :
     (pure loop_vars) ) : Id ((BitVec esize) × (BitVec esize) × (BitVec datasize)) )
   (pure result)
 
-/-- Type quantifiers: k_ex26555_ : Bool, datasize : Nat, elements : Nat, esize : Nat, esize ∈
+/-- Type quantifiers: k_ex26575_ : Bool, datasize : Nat, elements : Nat, esize : Nat, esize ∈
   {32, 64} ∧ elements ≥ 1 ∧ (elements * esize) = datasize -/
 def vector_arithmetic_binary_uniform_mul_fp_fused (datasize : Nat) (elements : Nat) (esize : Nat) (operand1 : (BitVec datasize)) (operand2 : (BitVec datasize)) (operand3 : (BitVec datasize)) (fpcr : (BitVec 32)) (sub_op : Bool) : (BitVec datasize) := Id.run do
   let result : (BitVec datasize) := (Zeros datasize)
@@ -805,7 +805,7 @@ def vector_arithmetic_binary_uniform_mul_fp_fused (datasize : Nat) (elements : N
     (pure loop_vars) ) : Id ((BitVec esize) × (BitVec esize) × (BitVec datasize)) )
   (pure result)
 
-/-- Type quantifiers: k_ex26631_ : Bool, k_ex26630_ : Bool, datasize : Nat, elements : Nat, esize :
+/-- Type quantifiers: k_ex26651_ : Bool, k_ex26650_ : Bool, datasize : Nat, elements : Nat, esize :
   Nat, esize ∈ {32, 64} ∧ elements ≥ 1 ∧ (elements * esize) = datasize -/
 def vector_arithmetic_binary_uniform_maxmin_fp_1985 (datasize : Nat) (elements : Nat) (esize : Nat) (operand1 : (BitVec datasize)) (operand2 : (BitVec datasize)) (fpcr : (BitVec 32)) (minimum : Bool) (pair : Bool) : (BitVec datasize) := Id.run do
   let result : (BitVec datasize) := (Zeros datasize)
@@ -837,7 +837,7 @@ def vector_arithmetic_binary_uniform_maxmin_fp_1985 (datasize : Nat) (elements :
     (pure loop_vars) ) : Id ((BitVec esize) × (BitVec esize) × (BitVec datasize)) )
   (pure result)
 
-/-- Type quantifiers: k_ex26729_ : Bool, k_ex26728_ : Bool, datasize : Nat, elements : Nat, esize :
+/-- Type quantifiers: k_ex26749_ : Bool, k_ex26748_ : Bool, datasize : Nat, elements : Nat, esize :
   Nat, esize ∈ {32, 64} ∧ elements ≥ 1 ∧ (elements * esize) = datasize -/
 def vector_arithmetic_binary_uniform_maxmin_fp_2008 (datasize : Nat) (elements : Nat) (esize : Nat) (operand1 : (BitVec datasize)) (operand2 : (BitVec datasize)) (fpcr : (BitVec 32)) (minimum : Bool) (pair : Bool) : (BitVec datasize) := Id.run do
   let result : (BitVec datasize) := (Zeros datasize)
@@ -887,7 +887,7 @@ def vector_arithmetic_unary_special_sqrt (datasize : Nat) (elements : Nat) (esiz
     (pure loop_vars) ) : Id ((BitVec esize) × (BitVec datasize)) )
   (pure result)
 
-/-- Type quantifiers: k_ex26876_ : Bool, datasize : Nat, elements : Nat, esize : Nat, esize ∈
+/-- Type quantifiers: k_ex26896_ : Bool, datasize : Nat, elements : Nat, esize : Nat, esize ∈
   {32, 64} ∧ elements ≥ 1 ∧ (elements * esize) = datasize -/
 def vector_arithmetic_unary_diffneg_fp (datasize : Nat) (elements : Nat) (esize : Nat) (operand : (BitVec datasize)) (neg : Bool) : (BitVec datasize) := Id.run do
   let result : (BitVec datasize) := (Zeros datasize)
@@ -935,13 +935,16 @@ def big_endian_reverse64_pure (value_name : (BitVec 64)) : (BitVec 64) :=
                 value_name 40 8) +++ ((BitVec.slice value_name 48 8) +++ (BitVec.slice value_name 56
                   8))))))))
 
-/-- Type quantifiers: k_ex26999_ : Bool -/
+/-- Type quantifiers: k_ex27019_ : Bool -/
 def str64_aligned_normal_write_memory_arguments_pure (big_endian : Bool) (paddress : (BitVec 52)) (pre_mem_data : (BitVec 64)) : ((BitVec 56) × (BitVec 64)) :=
   let write_data : (BitVec 64) :=
     if (big_endian : Bool)
     then (big_endian_reverse64_pure pre_mem_data)
     else pre_mem_data
   ((Sail.BitVec.zeroExtend paddress 56), write_data)
+
+def str64_no_device_write_ram_call_arguments_pure (default_ram : (BitVec 56)) (address : (BitVec 56)) (data : (BitVec 64)) : (Int × Int × (BitVec 56) × (BitVec 56) × (BitVec 64)) :=
+  (56, 8, default_ram, address, data)
 
 def undefined_MemBarrierOp (_ : Unit) : SailM MemBarrierOp := do
   (internal_pick
@@ -1211,7 +1214,7 @@ def undefined_PlainERETDecode (_ : Unit) : SailM PlainERETDecode := do
           pac := ← (undefined_bool ())
           use_key_a := ← (undefined_bool ()) })
 
-/-- Type quantifiers: k_ex27256_ : Bool -/
+/-- Type quantifiers: k_ex27278_ : Bool -/
 def decode64_plain_eret_pure (op_code : (BitVec 32)) (at_el0 : Bool) : PlainERETDecode :=
   let op4 : (BitVec 5) := (BitVec.slice op_code 0 5)
   let Rn : (BitVec 5) := (BitVec.slice op_code 5 5)
@@ -1287,8 +1290,8 @@ def decode64_system_write_vttbr_el2_pure (op_code : (BitVec 32)) : (Bool × Syst
   then (system_register_vttbr_el2_target_pure o0 op1 CRn CRm op2 Rt)
   else (false, SystemRegisterWriteTarget_VTTBR_EL2, Rt)
 
-/-- Type quantifiers: k_ex27955_ : Bool, k_ex27954_ : Bool, k_ex27953_ : Bool, k_ex27952_ : Bool, k_ex27951_
-  : Bool, k_ex27950_ : Bool -/
+/-- Type quantifiers: k_ex27977_ : Bool, k_ex27976_ : Bool, k_ex27975_ : Bool, k_ex27974_ : Bool, k_ex27973_
+  : Bool, k_ex27972_ : Bool -/
 def aarch64_sysregwrite_vttbr_el2_pure (at_el1 : Bool) (hcr_nv : Bool) (hcr_nv2 : Bool) (hcr_tge : Bool) (scr_ns : Bool) (scr_eel2 : Bool) (old_value : (BitVec 64)) (val_name : (BitVec 64)) : (Bool × (BitVec 64)) :=
   let redirected : Bool :=
     (at_el1 && (hcr_nv && (hcr_nv2 && ((! hcr_tge) && (scr_ns || scr_eel2)))))
@@ -1312,8 +1315,8 @@ def decode64_system_write_vtcr_el2_pure (op_code : (BitVec 32)) : (Bool × Syste
   then (system_register_vtcr_el2_target_pure o0 op1 CRn CRm op2 Rt)
   else (false, SystemRegisterWriteTarget_VTCR_EL2, Rt)
 
-/-- Type quantifiers: k_ex28077_ : Bool, k_ex28076_ : Bool, k_ex28075_ : Bool, k_ex28074_ : Bool, k_ex28073_
-  : Bool, k_ex28072_ : Bool -/
+/-- Type quantifiers: k_ex28099_ : Bool, k_ex28098_ : Bool, k_ex28097_ : Bool, k_ex28096_ : Bool, k_ex28095_
+  : Bool, k_ex28094_ : Bool -/
 def aarch64_sysregwrite_vtcr_el2_pure (at_el1 : Bool) (hcr_nv : Bool) (hcr_nv2 : Bool) (hcr_tge : Bool) (scr_ns : Bool) (scr_eel2 : Bool) (old_value : (BitVec 32)) (val_name : (BitVec 64)) : (Bool × (BitVec 32)) :=
   let redirected : Bool :=
     (at_el1 && (hcr_nv && (hcr_nv2 && ((! hcr_tge) && (scr_ns || scr_eel2)))))
@@ -1356,8 +1359,8 @@ def decode64_system_write_cntvoff_el2_pure (op_code : (BitVec 32)) : (Bool × Sy
   then (system_register_cntvoff_el2_target_pure o0 op1 CRn CRm op2 Rt)
   else (false, SystemRegisterWriteTarget_CNTVOFF_EL2, Rt)
 
-/-- Type quantifiers: k_ex28313_ : Bool, k_ex28312_ : Bool, k_ex28311_ : Bool, k_ex28310_ : Bool, k_ex28309_
-  : Bool, k_ex28308_ : Bool -/
+/-- Type quantifiers: k_ex28335_ : Bool, k_ex28334_ : Bool, k_ex28333_ : Bool, k_ex28332_ : Bool, k_ex28331_
+  : Bool, k_ex28330_ : Bool -/
 def aarch64_sysregwrite_cntvoff_el2_pure (at_el1 : Bool) (hcr_nv : Bool) (hcr_nv2 : Bool) (hcr_tge : Bool) (scr_ns : Bool) (scr_eel2 : Bool) (old_value : (BitVec 64)) (val_name : (BitVec 64)) : (Bool × (BitVec 64)) :=
   let redirected : Bool :=
     (at_el1 && (hcr_nv && (hcr_nv2 && ((! hcr_tge) && (scr_ns || scr_eel2)))))
@@ -1381,8 +1384,8 @@ def decode64_system_write_sp_el1_pure (op_code : (BitVec 32)) : (Bool × SystemR
   then (system_register_sp_el1_target_pure o0 op1 CRn CRm op2 Rt)
   else (false, SystemRegisterWriteTarget_SP_EL1, Rt)
 
-/-- Type quantifiers: k_ex28435_ : Bool, k_ex28434_ : Bool, k_ex28433_ : Bool, k_ex28432_ : Bool, k_ex28431_
-  : Bool, k_ex28430_ : Bool -/
+/-- Type quantifiers: k_ex28457_ : Bool, k_ex28456_ : Bool, k_ex28455_ : Bool, k_ex28454_ : Bool, k_ex28453_
+  : Bool, k_ex28452_ : Bool -/
 def aarch64_sysregwrite_sp_el1_pure (at_el1 : Bool) (hcr_nv : Bool) (hcr_nv2 : Bool) (hcr_tge : Bool) (scr_ns : Bool) (scr_eel2 : Bool) (old_value : (BitVec 64)) (val_name : (BitVec 64)) : (Bool × (BitVec 64)) :=
   let redirected : Bool :=
     (at_el1 && (hcr_nv && (hcr_nv2 && ((! hcr_tge) && (scr_ns || scr_eel2)))))
@@ -1444,8 +1447,8 @@ def decode64_system_write_hcr_el2_pure (op_code : (BitVec 32)) : (Bool × System
   then (system_register_hcr_el2_target_pure o0 op1 CRn CRm op2 Rt)
   else (false, SystemRegisterWriteTarget_HCR_EL2, Rt)
 
-/-- Type quantifiers: k_ex28785_ : Bool, k_ex28784_ : Bool, k_ex28783_ : Bool, k_ex28782_ : Bool, k_ex28781_
-  : Bool, k_ex28780_ : Bool -/
+/-- Type quantifiers: k_ex28807_ : Bool, k_ex28806_ : Bool, k_ex28805_ : Bool, k_ex28804_ : Bool, k_ex28803_
+  : Bool, k_ex28802_ : Bool -/
 def aarch64_sysregwrite_hcr_el2_pure (at_el1 : Bool) (old_hcr_nv : Bool) (old_hcr_nv2 : Bool) (old_hcr_tge : Bool) (scr_ns : Bool) (scr_eel2 : Bool) (old_value : (BitVec 64)) (val_name : (BitVec 64)) : (Bool × (BitVec 64)) :=
   let redirected : Bool :=
     (at_el1 && (old_hcr_nv && (old_hcr_nv2 && ((! old_hcr_tge) && (scr_ns || scr_eel2)))))
@@ -1484,7 +1487,7 @@ def undefined_ColdEntryRegisterSequenceResult (_ : Unit) : SailM ColdEntryRegist
           write6 := ← (undefined_SystemRegisterWriteTarget ())
           write7 := ← (undefined_SystemRegisterWriteTarget ()) })
 
-/-- Type quantifiers: k_ex28807_ : Bool, k_ex28806_ : Bool, k_ex28805_ : Bool, k_ex28804_ : Bool -/
+/-- Type quantifiers: k_ex28829_ : Bool, k_ex28828_ : Bool, k_ex28827_ : Bool, k_ex28826_ : Bool -/
 def eret_nv_trap_route_pure (have_nv_ext : Bool) (el2_enabled : Bool) (at_el1 : Bool) (hcr_nv : Bool) : Bool :=
   (((have_nv_ext && el2_enabled) && at_el1) && hcr_nv)
 
@@ -1493,14 +1496,14 @@ def undefined_PlainERETInputsAtEL2 (_ : Unit) : SailM PlainERETInputsAtEL2 := do
           target := ← (undefined_bitvector 64)
           spsr := ← (undefined_bitvector 32) })
 
-/-- Type quantifiers: k_ex28811_ : Bool, k_ex28810_ : Bool -/
+/-- Type quantifiers: k_ex28833_ : Bool, k_ex28832_ : Bool -/
 def aarch64_plain_eret_at_el2_inputs_pure (have_nv_ext : Bool) (el2_enabled : Bool) (state : ColdEntryRegisterState) : PlainERETInputsAtEL2 :=
   let hcr_nv : Bool := ((BitVec.access state.hcr_el2 42) == 1#1)
   { dedicated_nv_trap := (eret_nv_trap_route_pure have_nv_ext el2_enabled false hcr_nv)
     target := state.elr_el2
     spsr := state.spsr_el2 }
 
-/-- Type quantifiers: k_ex28815_ : Bool, k_ex28814_ : Bool -/
+/-- Type quantifiers: k_ex28837_ : Bool, k_ex28836_ : Bool -/
 def aarch64_cold_entry_register_sequence_at_el2_pure (old_state : ColdEntryRegisterState) (inputs : ColdEntryRegisterInputs) (scr_ns : Bool) (scr_eel2 : Bool) : ColdEntryRegisterSequenceResult :=
   let old_hcr_nv : Bool := ((BitVec.access old_state.hcr_el2 42) == 1#1)
   let old_hcr_nv2 : Bool := ((BitVec.access old_state.hcr_el2 45) == 1#1)
